A12Kernel.lean
@@ -149,6 +149,7 @@ import A12Kernel.Elaboration.StringComputationRunApplication
 import A12Kernel.Elaboration.NumberToStringComputationRun
 import A12Kernel.Elaboration.StringToNumberComputationRun
 import A12Kernel.Elaboration.ScalarComputationRun
+import A12Kernel.Elaboration.ScalarComputationRunResult
 import A12Kernel.Elaboration.EnumerationComputation
 import A12Kernel.Elaboration.EnumerationFirstFilledComputation
 import A12Kernel.Elaboration.NumericValidation
